some validators

lib/everparse/3d/EverParse3d.Actions.Base.fst
@@ -2,6 +2,7 @@ module EverParse3d.Actions.Base
 #lang-pulse
 friend EverParse3d.Kinds
 friend EverParse3d.Prelude
+open EverParse3d.ErrorCode
 open EverParse3d.Prelude
 open Pulse.Lib.Pervasives
 module I = EverParse3d.InputStream.Base
@@ -20,8 +21,8 @@ open EverParse3d.State
 
 let action
   (extra_state: state_dict)
-  (use_error_handler: bool)
   (a: Type0)
+  (use_error_handler: bool)
 =
   ctxt: app_ctxt ->
   error_handler_fn : (if use_error_handler then error_handler else unit) ->
@@ -41,12 +42,6 @@ let action
     )
 
 module LP = LowParse.Spec.Base
-
-[@@CMacro]
-let success = 0uy
-
-[@@CMacro]
-let action_failed = 1uy
 
 inline_for_extraction noextract
 let validate_with_action_t
@@ -76,11 +71,11 @@ let validate_with_action_t
     I.pts_to sl contents_sl v_sl' **
     forevery_state extra_state extra' **
     pure (
-      (res == action_failed ==> has_action) /\
+      (res == validator_error_action_failed ==> has_action) /\
       (not has_action ==> extra' == extra) /\
-      (U8.v res > U8.v action_failed ==> None? (LP.parse p v_sl)) /\
+      (U8.v res > U8.v validator_error_action_failed ==> None? (LP.parse p v_sl)) /\
       I.seq_is_suffix_of v_sl' v_sl /\
-      (res == success ==> (Some? (LP.parse p v_sl) /\ v_sl' == Seq.slice v_sl (snd (Some?.v (LP.parse p v_sl))) (Seq.length v_sl)))
+      (res == validator_success ==> (Some? (LP.parse p v_sl) /\ v_sl' == Seq.slice v_sl (snd (Some?.v (LP.parse p v_sl))) (Seq.length v_sl)))
   ))
 
 inline_for_extraction noextract
@@ -118,11 +113,53 @@ let validate_with_action_no_read
     pure (
       SZ.v v_pos <= Seq.length v_sl /\ (
       let pp = LP.parse p (Seq.slice v_sl (SZ.v v_pos) (Seq.length v_sl)) in
-      (res == action_failed ==> has_action) /\
+      (res == validator_error_action_failed ==> has_action) /\
       (not has_action ==> extra' == extra) /\
-      (U8.v res > U8.v action_failed ==> None? pp /\
-      (res == success ==> (Some? pp /\ SZ.v v_pos' == SZ.v v_pos + snd (Some?.v pp)))
-  ))))
+      (U8.v res > U8.v validator_error_action_failed ==> None? pp) /\
+      (res == validator_success ==> (Some? pp /\ SZ.v v_pos' == SZ.v v_pos + snd (Some?.v pp)))
+  )))
+
+inline_for_extraction noextract
+fn validate_eta
+      (#nz:bool)
+      (#wk: _)
+      (#k:parser_kind nz wk)
+      (#[@@@erasable] t:Type)
+      (#[@@@erasable] p:parser k t)
+      (#[@@@erasable] extra_state: state_dict)
+      (#has_action:bool)
+      (#use_error_handler:bool)
+      (v: validate_with_action_t p extra_state has_action use_error_handler)
+: validate_with_action_t p extra_state has_action use_error_handler
+=
+  (ctxt: _)
+  (error_handler_fn: _)
+  (sl: _)
+  (extra: _)
+  (contents_sl: _)
+  (v_sl: _)
+{
+  v ctxt error_handler_fn sl extra contents_sl v_sl
+}
+
+inline_for_extraction noextract
+fn act_with_comment
+      (s: string)
+      (extra_state: state_dict)
+      (#use_error_handler:bool)
+      (#res:Type)
+      (a: action extra_state res use_error_handler)
+: action extra_state res use_error_handler
+=
+  (ctxt: _)
+  (error_handler_fn: _)
+  (sl: _)
+  (contents_sl: _)
+  (v_sl: _)
+{
+  // TODO: add support for extracting compile-time comments in Pulse
+  a ctxt error_handler_fn sl contents_sl v_sl
+}
 
 inline_for_extraction
 let leaf_reader
@@ -151,18 +188,213 @@ let leaf_reader
     end
   ))
 
+inline_for_extraction noextract
+fn validate_with_success_action
+      (name: string)
+      (#nz:bool)
+      (#wk: _)
+      (#k1:parser_kind nz wk)
+      (#[@@@erasable] t1:Type)
+      (#[@@@erasable] p1:parser k1 t1)
+      (#[@@@erasable] extra: state_dict)
+      (#has_action:bool)
+      (#use_error_handler:bool)
+      (v1:validate_with_action_t p1 extra has_action use_error_handler)
+      (a:action extra bool use_error_handler)
+  : validate_with_action_t p1 extra true use_error_handler
+=
+  (ctxt: _)
+  (error_handler_fn: _)
+  (sl: _)
+  (extra: _)
+  (contents_sl: _)
+  (v_sl: _)
+{
+  let res_validate = v1 ctxt error_handler_fn sl extra contents_sl v_sl;
+  if (res_validate = validator_success) {
+    let res_action = a ctxt error_handler_fn sl _ _;
+    if (res_action) {
+      validator_success
+    } else {
+      validator_error_action_failed
+    }
+  } else {
+    res_validate
+  }
+}
+
+inline_for_extraction noextract
+fn validate_with_error_handler
+      (typename: string)
+      (fieldname: string)
+      (#nz: _)
+      (#wk: _)
+      (#k1:parser_kind nz wk)
+      (#[@@@erasable] t1: Type)
+      (#[@@@erasable] p1:parser k1 t1)
+      (#[@@@erasable] extra_state: state_dict)
+      (#has_action: _)
+      (#use_error_handler:bool)
+      (v1:validate_with_action_t p1 extra_state has_action use_error_handler)
+  : validate_with_action_t p1 extra_state has_action use_error_handler
+=
+  (ctxt: _)
+  (error_handler_fn: _)
+  (sl: _)
+  (extra: _)
+  (contents_sl: _)
+  (v_sl: _)
+{
+  let res = v1 ctxt error_handler_fn sl extra contents_sl v_sl;
+  if (res = validator_success) { // TODO: turn this `if ... else` into a non-terminal `if (res <> validator_success)` with an `ensures` clause
+    res
+  } else {
+    ((if use_error_handler then error_handler_fn else error_handler_macro) <: error_handler) typename fieldname (error_reason_of_result res) res ctxt sl _ _;
+    res
+  };
+}
+
+inline_for_extraction noextract
+fn validate_ret
+      (#extra_state: state_dict)
+      (#use_error_handler:bool)
+  : validate_with_action_t (parse_ret ()) extra_state false use_error_handler
+=
+  (ctxt: _)
+  (error_handler_fn: _)
+  (sl: _)
+  (extra: _)
+  (contents_sl: _)
+  (v_sl: _)
+{
+  validator_success
+}
+
+inline_for_extraction noextract
+fn validate_pair
+       (typename: string)
+       (name1: string)
+       (#nz1:_)
+       (#k1:parser_kind nz1 WeakKindStrongPrefix)
+       (#[@@@erasable] t1:Type)
+       (#[@@@erasable] p1:parser k1 t1)
+       (k1_const: bool)
+       (#[@@@erasable] extra_state: state_dict)
+       (#has_action1:bool)
+       (#use_error_handler:bool)
+       (v1:validate_with_action_t p1 extra_state has_action1 use_error_handler)
+       (#nz2:_)
+       (#wk2: _)
+       (#k2:parser_kind nz2 wk2)
+       (#[@@@erasable] t2:Type)
+       (#[@@@erasable] p2:parser k2 t2)
+       (k2_const: bool)
+       (#has_action2:bool)
+       (v2:validate_with_action_t p2 extra_state has_action2 use_error_handler)
+  : validate_with_action_t
+      (p1 `parse_pair` p2)
+      extra_state
+      (has_action1 || has_action2)
+      use_error_handler
+=
+  (ctxt: _)
+  (error_handler_fn: _)
+  (sl: _)
+  (extra: _)
+  (contents_sl: _)
+  (v_sl: _)
+{
+  LowParse.Spec.Combinators.nondep_then_eq p1 p2 v_sl;
+  let res1 = v1 ctxt error_handler_fn sl _ _ _;
+  if (res1 = validator_success) {
+    v2 ctxt error_handler_fn sl _ _ _
+  } else {
+    res1
+  }
+}
+
+
+#push-options "--z3rlimit 32"
+
+inline_for_extraction noextract
+fn validate_dep_pair_with_refinement_and_action
+      (p1_is_constant_size_without_actions: bool)
+      (name1: string)
+      (#nz1:_)
+      (#k1:parser_kind nz1 WeakKindStrongPrefix)
+      (#t1:Type)
+      (#[@@@erasable] p1:parser k1 t1)
+      (#[@@@erasable] extra_state: state_dict)
+      (#has_action1:bool)
+      (#use_error_handler:bool)
+      (v1:validate_with_action_no_read p1 extra_state has_action1 use_error_handler)
+      (r1: leaf_reader p1)
+      (f: t1 -> bool)
+      (a:t1 -> action extra_state bool use_error_handler)
+      (#nz2:_)
+      (#wk2: _)
+      (#k2:parser_kind nz2 wk2)
+      (#[@@@erasable] t2:refine _ f -> Type)
+      (#[@@@erasable] p2:(x:refine _ f -> parser k2 (t2 x)))
+      (#has_action2:bool)
+      (v2:(x:refine _ f -> validate_with_action_t (p2 x) extra_state has_action2 use_error_handler))
+  : validate_with_action_t
+      ((p1 `parse_filter` f) `parse_dep_pair` p2)
+      extra_state
+      true
+      use_error_handler
+=
+  (ctxt: _)
+  (error_handler_fn: _)
+  (sl: _)
+  (extra: _)
+  (contents_sl: _)
+  (v_sl: _)
+{
+  LowParse.Spec.Combinators.parse_dtuple2_eq (parse_filter p1 f) p2 v_sl;
+  LowParse.Spec.Combinators.parse_filter_eq p1 f v_sl;
+  let mut pos = 0sz;
+  let res_key = v1 ctxt error_handler_fn sl pos _ _ _ _;
+  if (res_key = validator_success) {
+    let val_key = r1 sl _ _;
+    if (f val_key) {
+      let res_action = a val_key ctxt error_handler_fn sl _ _;
+      if (res_action) {
+      	 v2 val_key ctxt error_handler_fn sl _ _ _;
+      } else {
+        validator_error_action_failed
+      }
+    } else {
+      validator_error_constraint_failed
+    }
+  } else {
+    res_key
+  }
+}
+
+#pop-options
+
 
 noextract
 inline_for_extraction
-let action_bind
+fn action_bind
       (name: string)
       (#extra_state: state_dict)
       (#use_error_handler:bool)
       (#a: Type)
-      (f: action extra_state use_error_handler a)
-      (#b:Type) (g: (a -> action extra_state use_error_handler b))
-: Tot (action extra_state use_error_handler b)
-= admit ()
+      (f: action extra_state a use_error_handler)
+      (#b:Type) (g: (a -> action extra_state b use_error_handler))
+: action extra_state b use_error_handler
+=
+  (ctxt: _)
+  (error_handler_fn: _)
+  (sl: _)
+  (contents_sl: _)
+  (v_sl: _)
+{
+  let resf = f ctxt error_handler_fn sl _ _;
+  g resf ctxt error_handler_fn sl _ _
+}
 
 noextract
 inline_for_extraction
@@ -170,10 +402,10 @@ let action_weaken
       (#d1: state_dict)
       (#use_error_handler:bool)
       (#a: Type)
-      (f: action d1 use_error_handler a)
+      (f: action d1 a use_error_handler)
       (d2: state_dict)
       (d2_extends: squash (state_dict_weaken_prop d1 d2))
-: Tot (action d2 use_error_handler a)
+: Tot (action d2 a use_error_handler)
 = admit ()
 
 noextract
@@ -181,7 +413,7 @@ inline_for_extraction
 let action_deref
       (name: string)
       (#a:Type) (x:ref a) (#use_error_handler: bool)
-: Tot (action (state_dict_singleton name (pts_to x #1.0R)) use_error_handler a)
+: Tot (action (state_dict_singleton name (pts_to x #1.0R)) a use_error_handler)
 = admit ()
 
 noextract
@@ -189,7 +421,7 @@ inline_for_extraction
 let action_assignment
       (name: string)
       (#a:Type) (x:ref a) (w: a) (#use_error_handler: bool)
-: Tot (action (state_dict_singleton name (pts_to x #1.0R)) use_error_handler a)
+: Tot (action (state_dict_singleton name (pts_to x #1.0R)) a use_error_handler)
 = admit ()
 
 (*
